refactoring (affine)

theories/examples/affine_lang/lang.v
@@ -1,6 +1,7 @@
 From gitrees Require Export lang_generic gitree program_logic.
-From gitrees.input_lang Require Import lang interp.
-From gitrees.examples Require Import store pairs.
+From gitrees.examples.input_lang Require Import lang interp.
+From gitrees.effects Require Import store.
+From gitrees.lib Require Import pairs.
 
 (* for namespace sake *)
 Module io_lang.
@@ -14,14 +15,12 @@ Module io_lang.
     input_lang.interp.interp_expr rs e (ı_scope rs).
 End io_lang.
 
-From gitrees Require Export lang_affine.
+Require Import Binding.Resolver Binding.Lib Binding.Set Binding.Auto Binding.Env.
 
 Inductive ty :=
   tBool | tInt | tUnit
 | tArr (τ1 τ2 : ty) | tPair (τ1 τ2 : ty)
 | tRef (τ : ty).
-
-Local Notation tyctx := (tyctx ty).
 
 Inductive ty_conv : ty → io_lang.ty → Type :=
 | ty_conv_bool : ty_conv tBool Tnat
@@ -32,19 +31,19 @@ Inductive ty_conv : ty → io_lang.ty → Type :=
   ty_conv (tArr τ1 τ2) (Tarr (Tarr Tnat t1) t2)
 .
 
-Inductive expr : scope → Type :=
-| LitBool (b : bool) {S} : expr S
-| LitNat (n : nat) {S} : expr S
-| LitUnit {S} : expr S
-| Lam {S} : expr (tt::S) → expr S
-| Var {S} : var S → expr S
-| App {S1 S2} : expr S1 → expr S2 → expr (S1++S2)
-| EPair {S1 S2} : expr S1 → expr S2 → expr (S1++S2)
-| EDestruct {S1 S2} : expr S1 → expr (()::()::S2) → expr (S1++S2)
-| Alloc {S} : expr S → expr S
-| Replace {S1 S2} : expr S1 → expr S2 → expr (S1++S2)
-| Dealloc {S} : expr S → expr S
-| EEmbed {τ1 τ1' S} : io_lang.expr Empty_set → ty_conv τ1 τ1' → expr S
+Inductive expr : ∀ (S : Set), Type :=
+| LitBool {S : Set} (b : bool) : expr S
+| LitNat {S : Set} (n : nat) : expr S
+| LitUnit {S : Set} : expr S
+| Lam {S : Set} : expr (inc S) → expr S
+| Var {S : Set} : S → expr S
+| App {S1 S2 : Set} : expr S1 → expr S2 → expr (sum S1 S2)
+| EPair {S1 S2 : Set} : expr S1 → expr S2 → expr (sum S1 S2)
+| EDestruct {S1 S2 : Set} : expr S1 → expr (inc (inc S2)) → expr (sum S1 S2)
+| Alloc {S : Set} : expr S → expr S
+| Replace {S1 S2 : Set} : expr S1 → expr S2 → expr (sum S1 S2)
+| Dealloc {S : Set} : expr S → expr S
+| EEmbed {S : Set} {τ1 τ1'} : io_lang.expr Empty_set → ty_conv τ1 τ1' → expr S
 .
 
 Section affine.
@@ -64,9 +63,11 @@ Section affine.
       λit _, IF (READ ℓ) (Err OtherError)
                          (SEQ (WRITE ℓ (Ret 1)) e).
   Solve All Obligations with first [solve_proper|solve_proper_please].
+
   Program Definition thunkedV : IT -n> locO -n> ITV := λne e ℓ,
       FunV $ Next (λne _, IF (READ ℓ) (Err OtherError) (SEQ (WRITE ℓ (Ret 1)) e)).
   Solve All Obligations with first [solve_proper|solve_proper_please].
+
   #[export] Instance thunked_into_val e l : IntoVal (thunked e l) (thunkedV e l).
   Proof.
     unfold IntoVal. simpl. f_equiv. f_equiv. intro. done.
@@ -75,45 +76,52 @@ Section affine.
   Program Definition Thunk : IT -n> IT := λne e,
       ALLOC (Ret 0) (thunked e).
   Solve All Obligations with first [solve_proper|solve_proper_please].
+
   Program Definition Force : IT -n> IT := λne e, e ⊙ (Ret 0).
 
   Local Open Scope type.
 
   Definition interp_litbool {A} (b : bool)  : A -n> IT := λne _,
-    Ret (if b then 1 else 0).
+      Ret (if b then 1 else 0).
+
   Definition interp_litnat {A}  (n : nat) : A -n> IT := λne _,
-    Ret n.
+      Ret n.
+
   Definition interp_litunit {A} : A -n> IT := λne _, Ret tt.
+
   Program Definition interp_pair {A1 A2} (t1 : A1 -n> IT) (t2 : A2 -n> IT)
-    : A1*A2 -n> IT := λne env,
+    : A1 * A2 -n> IT := λne env,
     pairIT (t1 env.1) (t2 env.2).  (* we don't need to evaluate the pair here, i.e. lazy pairs? *)
   Next Obligation. solve_proper_please. Qed.
-  Program Definition interp_lam {A : ofe} (b : (IT * A) -n> IT) : A -n> IT := λne env,
-    λit x, b (x,env).
-  Solve All Obligations with solve_proper_please.
+
+  Program Definition interp_lam {S : Set} (b : @interp_scope F R _ (inc S) -n> IT) : @interp_scope F R _ S -n> IT := λne env, (λit x, (b (@extend_scope F R _ _ env x))).
+  Next Obligation.
+    intros; repeat intro; repeat f_equiv; assumption.
+  Qed.
+  Next Obligation.
+    intros; repeat intro; repeat f_equiv; intro; simpl;
+      f_equiv; intro z; simpl.
+    destruct z; done.
+  Qed.
+
   Program Definition interp_app {A1 A2 : ofe} (t1 : A1 -n> IT) (t2 : A2 -n> IT)
     : A1*A2 -n> IT := λne env,
     LET (t2 env.2) $ λne x,
     LET (t1 env.1) $ λne f,
     APP' f (Thunk x).
   Solve All Obligations with solve_proper_please.
-  Program Definition interp_destruct {A1 A2 : ofe}
-       (ps : A1 -n> IT) (t : IT*(IT*A2) -n> IT)
-    : A1*A2 -n> IT := λne env,
-    LET (ps env.1) $ λne ps,
-    LET (Thunk (projIT1 ps)) $ λne x,
-    LET (Thunk (projIT2 ps)) $ λne y,
-    t (x, (y, env.2)).
-  Solve All Obligations with solve_proper_please.
+
   Program Definition interp_alloc {A} (α : A -n> IT) : A -n> IT := λne env,
     LET (α env) $ λne α, ALLOC α Ret.
   Solve All Obligations with solve_proper_please.
+
   Program Definition interp_replace {A1 A2} (α : A1 -n> IT) (β : A2 -n> IT) : A1*A2 -n> IT := λne env,
     LET (β env.2) $ λne β,
     flip get_ret (α env.1) $ λne (l : loc),
     LET (READ l) $ λne γ,
     SEQ (WRITE l β) (pairIT γ (Ret l)).
   Solve All Obligations with solve_proper_please.
+
   Program Definition interp_dealloc {A} (α : A -n> IT) : A -n> IT := λne env,
     get_ret DEALLOC (α env).
   Solve All Obligations with solve_proper_please.
@@ -154,6 +162,35 @@ Section affine.
     | ty_conv_fun conv1 conv2 => glue_from_affine_fun (glue_from_affine conv2) (glue_to_affine conv1)
     end.
 
+  Program Definition interp_destruct {S1 S2 : Set}
+    (ps : @interp_scope F R _ S1 -n> IT)
+    (t : (@interp_scope F R _ (inc (inc S2)) -n> IT))
+    : (@interp_scope F R _ S1 * @interp_scope F R _ S2) -n> IT
+    :=  λne env,
+      LET (ps env.1) $ λne z,
+      LET (Thunk (projIT1 z)) $ λne x,
+      LET (Thunk (projIT2 z)) $ λne y,
+      (t (@extend_scope F R _ _ (@extend_scope F R _ _ env.2 y) x)).
+  Next Obligation.
+    intros; repeat intro; repeat f_equiv; assumption.
+  Qed.
+  Next Obligation.
+    intros; repeat intro; repeat f_equiv; intro; simpl; f_equiv; intro A; simpl.
+    destruct A as [| [|]]; [assumption | reflexivity | reflexivity].
+  Qed.
+  Next Obligation.
+    intros; repeat intro; repeat f_equiv; first assumption.
+    intro; simpl; f_equiv; intro; simpl.
+    repeat f_equiv; intro; simpl; repeat f_equiv; intro; simpl.
+    repeat f_equiv; assumption.
+  Qed.
+  Next Obligation.
+    intros; repeat intro; repeat f_equiv; first assumption.
+    intro; simpl; f_equiv; intro; simpl.
+    repeat f_equiv; intro; simpl; repeat f_equiv; intro A; simpl.
+    destruct A as [| [|]]; [reflexivity | reflexivity |].
+    repeat f_equiv; assumption.
+  Qed.
 
   Fixpoint interp_expr {S} (e : expr S) : interp_scope S -n> IT :=
     match e with
@@ -162,12 +199,16 @@ Section affine.
     | LitUnit   => interp_litunit
     | Var v     => Force ◎ interp_var v
     | Lam e    => interp_lam (interp_expr e)
-    | App e1 e2 => interp_app (interp_expr e1) (interp_expr e2) ◎ interp_scope_split
-    | EPair e1 e2 => interp_pair (interp_expr e1) (interp_expr e2) ◎ interp_scope_split
-    | EDestruct e1 e2 => interp_destruct (interp_expr e1) (interp_expr e2) ◎ interp_scope_split
+    | App e1 e2 =>
+        interp_app (interp_expr e1) (interp_expr e2) ◎ interp_scope_split
+    | EPair e1 e2 =>
+        interp_pair (interp_expr e1) (interp_expr e2) ◎ interp_scope_split
+    | EDestruct e1 e2 =>
+        interp_destruct (interp_expr e1) (interp_expr e2) ◎ interp_scope_split
     | Alloc e => interp_alloc (interp_expr e)
     | Dealloc e => interp_dealloc (interp_expr e)
-    | Replace e1 e2 => interp_replace (interp_expr e1) (interp_expr e2) ◎ interp_scope_split
+    | Replace e1 e2 =>
+        interp_replace (interp_expr e1) (interp_expr e2) ◎ interp_scope_split
     | EEmbed e tconv =>
         constO $ glue_to_affine tconv (io_lang.interp_closed _ e)
     end.
