theories/effects/store.v
@@ -1,4 +1,3 @@
-From Equations Require Import Equations.
 From iris.algebra Require Import gmap excl auth gmap_view.
 From iris.proofmode Require Import classes tactics.
 From iris.base_logic Require Import algebra.
