theories/examples/affine_lang/logrel1.v
@@ -1,0 +1,931 @@
+(** Unary (Kripke) logical relation for the affine lang *)
+From gitrees Require Export gitree program_logic.
+From gitrees.examples.affine_lang Require Import lang.
+From gitrees.effects Require Import store.
+From gitrees.lib Require Import pairs.
+Require Import iris.algebra.gmap.
+Require Import stdpp.finite.
+
+Require Import Binding.Resolver Binding.Lib Binding.Set Binding.Auto Binding.Env.
+
+Lemma fin_to_set_sum {S1 S2 : Set} `{EqDecision S1} `{EqDecision S2} `{EqDecision (S1 + S2)}
+  `{Finite S1} `{Finite S2} `{Finite (S1 + S2)}
+  `{Countable S1} `{Countable S2} `{Countable (S1 + S2)}
+  : let A1 : gset S1 := (fin_to_set S1) in
+    let A2 : gset (S1 + S2) := set_map (inl : S1 → S1 + S2) A1 in
+    let B1 : gset S2 := (fin_to_set S2) in
+    let B2 : gset (S1 + S2) := set_map (inr : S2 → S1 + S2) B1 in
+    let C : gset (S1 + S2) := fin_to_set (S1 + S2) in
+    C = A2 ∪ B2.
+Proof.
+  apply set_eq.
+  intros [x|x]; simpl; split; intros _.
+  - apply elem_of_union; left.
+    apply elem_of_map_2.
+    apply elem_of_fin_to_set.
+  - apply elem_of_fin_to_set.
+  - apply elem_of_union; right.
+    apply elem_of_map_2.
+    apply elem_of_fin_to_set.
+  - apply elem_of_fin_to_set.
+Qed.
+
+Lemma fin_to_set_empty :
+  let A : gset ∅ := fin_to_set ∅ in
+  let B : gset ∅ := empty in
+  A = B.
+Proof.
+  apply set_eq; intros [].
+Qed.
+
+Section InstSum.
+  Global Instance EqDecisionLeft {S1 S2 : Set} {H : EqDecision (S1 + S2)} : EqDecision S1.
+  Proof.
+    intros x y.
+    destruct (decide (inl x = inl y)) as [G | G];
+      [left; by inversion G | right; intros C; by subst].
+  Qed.
+
+  Global Instance EqDecisionRight {S1 S2 : Set} {H : EqDecision (S1 + S2)} : EqDecision S2.
+  Proof.
+    intros x y.
+    destruct (decide (inr x = inr y)) as [G | G];
+      [left; by inversion G | right; intros C; by subst].
+  Qed.
+
+  Global Instance FiniteLeft {S1 S2 : Set} `{EqDecision S1}
+    `{EqDecision (S1 + S2)} `{Finite (S1 + S2)}
+    : Finite S1.
+  Proof.
+    unshelve econstructor.
+    - apply (foldr (λ x acc, match x with
+                             | inl x => x :: acc
+                             | inr _ => acc
+                             end) [] (enum (S1 + S2))).
+    - set (l := enum (S1 + S2)).
+      assert (NoDup l) as K; first apply NoDup_enum.
+      clearbody l.
+      induction l as [| a l IH]; first constructor.
+      destruct a as [a | a]; simpl.
+      + constructor.
+        * intros C.
+          assert (inl a ∈ l) as C'.
+          {
+            clear -C.
+            induction l as [| b l IH]; first inversion C.
+            destruct b as [b | b]; simpl.
+            - rewrite foldr_cons in C.
+              rewrite elem_of_cons in C.
+              destruct C as [-> | C].
+              + apply elem_of_cons.
+                by left.
+              + right.
+                apply IH.
+                apply C.
+            - apply elem_of_cons.
+              right.
+              rewrite foldr_cons in C.
+              apply IH.
+              apply C.
+          }
+          by inversion K.
+        * apply IH.
+          by inversion K.
+      + apply IH.
+        by inversion K.
+    - intros x.
+      set (l := enum (S1 + S2)).
+      assert (inl x ∈ l) as K; first apply elem_of_enum.
+      clearbody l.
+      induction l as [| a l IH]; first inversion K.
+      destruct a as [a | a]; simpl.
+      + rewrite elem_of_cons in K.
+        destruct K as [K | K].
+        * inversion K; subst.
+          apply elem_of_cons; by left.
+        * apply elem_of_cons; right; by apply IH.
+      + rewrite elem_of_cons in K.
+        destruct K as [K | K]; first inversion K.
+        by apply IH.
+  Qed.
+
+  Global Instance FiniteRight {S1 S2 : Set} `{EqDecision S2}
+    `{EqDecision (S1 + S2)} `{H : Finite (S1 + S2)}
+    : Finite S2.
+  Proof.
+    unshelve econstructor.
+    - apply (foldr (λ x acc, match x with
+                             | inl _ => acc
+                             | inr x => x :: acc
+                             end) [] (enum (S1 + S2))).
+    - set (l := enum (S1 + S2)).
+      assert (NoDup l) as K; first apply NoDup_enum.
+      clearbody l.
+      induction l as [| a l IH]; first constructor.
+      destruct a as [a | a]; simpl.
+      + apply IH.
+        by inversion K.
+      + constructor.
+        * intros C.
+          assert (inr a ∈ l) as C'.
+          {
+            clear -C.
+            induction l as [| b l IH]; first inversion C.
+            destruct b as [b | b]; simpl.
+            - apply elem_of_cons.
+              right.
+              rewrite foldr_cons in C.
+              apply IH.
+              apply C.
+            - rewrite foldr_cons in C.
+              rewrite elem_of_cons in C.
+              destruct C as [-> | C].
+              + apply elem_of_cons.
+                by left.
+              + right.
+                apply IH.
+                apply C.
+          }
+          by inversion K.
+        * apply IH.
+          by inversion K.
+    - intros x.
+      set (l := enum (S1 + S2)).
+      assert (inr x ∈ l) as K; first apply elem_of_enum.
+      clearbody l.
+      induction l as [| a l IH]; first inversion K.
+      destruct a as [a | a]; simpl.
+      + rewrite elem_of_cons in K.
+        destruct K as [K | K]; first inversion K.
+        by apply IH.
+      + rewrite elem_of_cons in K.
+        destruct K as [K | K].
+        * inversion K; subst.
+          apply elem_of_cons; by left.
+        * apply elem_of_cons; right; by apply IH.
+  Qed.
+
+End InstSum.
+
+Section InstInc.
+  Context (S : Set).
+
+  Global Instance EqDecisionIncN {HS : EqDecision S} (n : nat) : EqDecision (Init.Nat.iter n inc S).
+  Proof using S.
+    induction n; simpl.
+    - apply _.
+    - intros [|x] [|y].
+      + by left.
+      + by right.
+      + by right.
+      + destruct (decide (x = y)) as [-> |]; first by left.
+        right; by inversion 1.
+  Qed.
+
+  Global Instance EqDecisionInc {HS : EqDecision S} : EqDecision (inc S).
+  Proof using S.
+    assert (inc S = Init.Nat.iter 1 inc S) as ->; first done.
+    by apply EqDecisionIncN.
+  Qed.
+
+  Global Instance FiniteIncN {HS : EqDecision S} (HF : Finite S) (n : nat) {HS' : EqDecision (Init.Nat.iter n inc S)} : Finite (Init.Nat.iter n inc S).
+  Proof using S.
+    induction n.
+    - apply (@surjective_finite S HS HF _ _ id).
+      apply _.
+    - simpl.
+      unshelve eapply (@surjective_finite (option (Init.Nat.iter n inc S))); simpl in *.
+      + intros [x |].
+        * apply (VS x).
+        * apply VZ.
+      + apply _.
+      + intros [| x]; simpl.
+        * exists None; reflexivity.
+        * exists (Some x); reflexivity.
+  Qed.
+
+  Global Instance FiniteInc {HS : EqDecision S} (HF : Finite S) (HE : EqDecision (inc S)) : Finite (inc S).
+  Proof using S.
+    assert (J : @Finite (Init.Nat.iter 1 inc S) HE).
+    { apply FiniteIncN, HF. }
+    simpl in J.
+    apply J.
+  Qed.
+
+End InstInc.
+
+Definition sum_map' {A B C : Set} (f : A → C) (g : B → C) : sum A B → C :=
+  λ x, match x with | inl x' => f x' | inr x' => g x' end.
+
+Inductive typed : forall {S : Set}, (S → ty) → expr S → ty → Prop :=
+(** functions *)
+| typed_Var {S : Set} (Ω : S → ty) (v : S)  :
+  typed Ω (Var v) (Ω v)
+| typed_Lam {S : Set} (Ω : S → ty) (τ1 τ2 : ty) (e : expr (inc S) ) :
+  typed (Ω ▹ τ1) e τ2 →
+  typed Ω (Lam e) (tArr τ1 τ2)
+| typed_App {S1 S2 : Set} (Ω1 : S1 → ty) (Ω2 : S2 → ty) (τ1 τ2 : ty) e1 e2 :
+  typed Ω1 e1 (tArr τ1 τ2) →
+  typed Ω2 e2 τ1 →
+  typed (sum_map' Ω1 Ω2) (App e1 e2) τ2
+(** pairs *)
+| typed_Pair {S1 S2 : Set} (Ω1 : S1 → ty) (Ω2 : S2 → ty) (τ1 τ2 : ty) e1 e2 :
+  typed Ω1 e1 τ1 →
+  typed Ω2 e2 τ2 →
+  typed (sum_map' Ω1 Ω2) (EPair e1 e2) (tPair τ1 τ2)
+| typed_Destruct {S1 S2 : Set} (Ω1 : S1 → ty) (Ω2 : S2 → ty) (τ1 τ2 τ : ty)
+  (e1 : expr S1) (e2 : expr (inc (inc S2))) :
+  typed Ω1 e1 (tPair τ1 τ2) →
+  typed ((Ω2 ▹ τ2) ▹ τ1) e2 τ →
+  typed (sum_map' Ω1 Ω2) (EDestruct e1 e2) τ
+(** references *)
+| typed_Alloc {S : Set} (Ω : S → ty) τ e :
+  typed Ω e τ →
+  typed Ω (Alloc e) (tRef τ)
+| typed_Replace {S1 S2 : Set} (Ω1 : S1 → ty) (Ω2 : S2 → ty) (τ1 τ2 : ty) e1 e2 :
+  typed Ω1 e1 (tRef τ1) →
+  typed Ω2 e2 τ2 →
+  typed (sum_map' Ω1 Ω2) (Replace e1 e2) (tPair τ1 (tRef τ2))
+| typed_Dealloc {S : Set} (Ω : S → ty) e τ :
+  typed Ω e (tRef τ) →
+  typed Ω (Dealloc e) tUnit
+(** literals *)
+| typed_Nat {S : Set} (Ω : S → ty) n :
+  typed Ω (LitNat n) tInt
+| typed_Bool {S : Set} (Ω : S → ty) b :
+  typed Ω (LitBool b) tBool
+| typed_Unit {S : Set} (Ω : S → ty) :
+  typed Ω LitUnit tUnit
+.
+
+Section logrel.
+  Context {sz : nat}.
+  Variable rs : gReifiers NotCtxDep sz.
+  Context `{!subReifier reify_store rs}.
+  Context `{!subReifier input_lang.interp.reify_io rs}.
+  Notation F := (gReifiers_ops NotCtxDep rs).
+  Context {R} `{!Cofe R}.
+  Context `{!SubOfe natO R}.
+  Context `{!SubOfe unitO R}.
+  Context `{!SubOfe locO R}.
+  Notation IT := (IT F R).
+  Notation ITV := (ITV F R).
+  Context `{!invGS Σ, !stateG rs R Σ, !heapG rs R Σ}.
+  Notation iProp := (iProp Σ).
+
+  (* parameters for the kripke logical relation *)
+  Variable s : stuckness.
+  Context `{A:ofe}.
+  Variable (P : A -n> iProp).
+  Local Notation expr_pred := (expr_pred s rs P).
+
+  (* interpreting tys *)
+  Program Definition protected (Φ : ITV -n> iProp) : ITV -n> iProp := λne αv,
+    (WP@{rs} Force (IT_of_V αv) @ s {{ Φ }})%I.
+  Solve All Obligations with solve_proper_please.
+  Program Definition interp_tbool : ITV -n> iProp := λne αv,
+    (αv ≡ RetV 0 ∨ αv ≡ RetV 1)%I.
+  Solve All Obligations with solve_proper_please.
+  Program Definition interp_tnat : ITV -n> iProp := λne αv,
+    (∃ n : nat, αv ≡ RetV n)%I.
+  Solve All Obligations with solve_proper_please.
+  Program Definition interp_tunit : ITV -n> iProp := λne αv,
+    (αv ≡ RetV ())%I.
+  Solve All Obligations with solve_proper_please.
+  Program Definition interp_tpair (Φ1 Φ2 : ITV -n> iProp) : ITV -n> iProp := λne αv,
+    (∃ β1v β2v, IT_of_V αv ≡ pairITV (IT_of_V β1v) (IT_of_V β2v) ∗
+                  Φ1 β1v ∗ Φ2 β2v)%I.
+  Solve All Obligations with solve_proper_please.
+  Program Definition interp_tarr (Φ1 Φ2 : ITV -n> iProp) : ITV -n> iProp := λne αv,
+    (∀ βv, Φ1 βv -∗ expr_pred ((IT_of_V αv) ⊙ (Thunk (IT_of_V βv))) Φ2)%I.
+  Solve All Obligations with solve_proper_please.
+
+  Program Definition interp_ref (Φ : ITV -n> iProp) : ITV -n> iProp := λne αv,
+    (∃ (l : loc), αv ≡ RetV l ∗ ∃ βv, pointsto l (IT_of_V βv) ∗ Φ βv)%I.
+  Solve All Obligations with solve_proper_please.
+
+  Fixpoint interp_ty (τ : ty) : ITV -n> iProp :=
+    match τ with
+    | tBool => interp_tbool
+    | tUnit => interp_tunit
+    | tInt  => interp_tnat
+    | tPair τ1 τ2 => interp_tpair (interp_ty τ1) (interp_ty τ2)
+    | tArr τ1 τ2 => interp_tarr  (interp_ty τ1) (interp_ty τ2)
+    | tRef τ => interp_ref (interp_ty τ)
+    end.
+
+  Program Definition ssubst_valid {S : Set} `{!EqDecision S} `{!Finite S}
+    (Ω : S → ty) (ss : interp_scope S) : iProp
+    := ([∗ set] x ∈ (fin_to_set S),
+         (expr_pred (ss x) (protected (interp_ty (Ω x))))%I).
+
+  Definition valid1 {S : Set} `{!EqDecision S} `{!Finite S} (Ω : S → ty)
+    (α : interp_scope S -n> IT) (τ : ty) : iProp :=
+    ∀ ss, heap_ctx
+          -∗ (ssubst_valid Ω ss)
+          -∗ expr_pred (α ss) (interp_ty τ).
+
+  Lemma ssubst_valid_empty (αs : interp_scope ∅) :
+    ⊢ ssubst_valid □ αs.
+  Proof.
+    iStartProof.
+    unfold ssubst_valid.
+    match goal with
+    | |- context G [big_opS ?a ?b ?c] => assert (c = empty) as ->
+    end.
+    { apply set_eq; intros []. }
+    by iApply big_sepS_empty.
+  Qed.
+
+  Lemma ssubst_valid_app
+    {S1 S2 : Set} `{!EqDecision S1} `{!Finite S1}
+    `{!EqDecision S2} `{!Finite S2}
+    `{!EqDecision (S1 + S2)} `{!Finite (S1 + S2)}
+    (Ω1 : S1 → ty) (Ω2 : S2 → ty)
+    (αs : interp_scope (sum S1 S2)) :
+    (ssubst_valid (sum_map' Ω1 Ω2) αs) ⊢
+    (ssubst_valid Ω1 (interp_scope_split αs).1)
+    ∗ (ssubst_valid Ω2 (interp_scope_split αs).2).
+  Proof.
+    iIntros "H".
+    rewrite /ssubst_valid fin_to_set_sum big_sepS_union; first last.
+    {
+      apply elem_of_disjoint.
+      intros [x | x].
+      - rewrite !elem_of_list_to_set.
+        intros _ H2.
+        apply elem_of_list_fmap_2 in H2.
+        destruct H2 as [y [H2 H2']]; inversion H2.
+      - rewrite !elem_of_list_to_set.
+        intros H1 _.
+        apply elem_of_list_fmap_2 in H1.
+        destruct H1 as [y [H1 H1']]; inversion H1.
+    }
+    iDestruct "H" as "(H1 & H2)".
+    iSplitL "H1".
+    - rewrite big_opS_list_to_set; first last.
+      {
+        apply NoDup_fmap.
+        - intros ??; by inversion 1.
+        - apply NoDup_elements.
+      }
+      rewrite big_sepL_fmap /=.
+      rewrite big_sepS_elements.
+      iFrame "H1".
+    - rewrite big_opS_list_to_set; first last.
+      {
+        apply NoDup_fmap.
+        - intros ??; by inversion 1.
+        - apply NoDup_elements.
+      }
+      rewrite big_sepL_fmap /=.
+      rewrite big_sepS_elements.
+      iFrame "H2".
+  Qed.
+
+  Lemma ssubst_valid_cons {S : Set} `{!EqDecision S} `{!Finite S}
+    (Ω : S → ty) (αs : interp_scope S) τ t :
+    ssubst_valid Ω αs ∗ expr_pred t (protected (interp_ty τ)) ⊢ ssubst_valid (Ω ▹ τ) (extend_scope αs t).
+  Proof.
+    iIntros "(H & G)".
+    rewrite /ssubst_valid.
+    pose (Y := let A := {[VZ]} : @gset (leibnizO (inc S)) _ finite_countable in
+               let B := fin_to_set (leibnizO S) : gset (leibnizO S) in
+               let C := set_map (VS : S → inc S) B
+                   : gset (inc S) in A ∪ C).
+    assert (fin_to_set (inc S) = Y) as ->.
+    {
+      subst Y; simpl.
+      apply set_eq.
+      intros [| x].
+      - split.
+        + intros _; apply elem_of_union; left.
+          by apply elem_of_singleton.
+        + intros _; apply elem_of_fin_to_set.
+      - split.
+        + intros _; apply elem_of_union; right.
+          apply elem_of_map_2, elem_of_fin_to_set.
+        + intros H.
+          apply elem_of_fin_to_set.
+    }
+    subst Y; simpl.
+    rewrite big_sepS_union; first last.
+    {
+      apply elem_of_disjoint.
+      intros [| x].
+      - rewrite !elem_of_list_to_set.
+        intros _ H2.
+        apply elem_of_list_fmap_2 in H2.
+        destruct H2 as [y [H2 H2']]; inversion H2.
+      - rewrite !elem_of_list_to_set.
+        intros H1 _.
+        apply elem_of_singleton_1 in H1.
+        inversion H1.
+    }
+    iSplitL "G".
+    - rewrite big_opS_singleton.
+      iFrame "G".
+    - erewrite big_opS_set_map.
+      + iFrame "H".
+      + intros ?? H; by inversion H.
+  Qed.
+
+  Lemma ssubst_valid_lookup {S : Set} `{!EqDecision S} `{!Finite S}
+    (Ω : S → ty) (αs : interp_scope S) x :
+    ssubst_valid Ω αs ⊢ expr_pred (αs x) (protected (interp_ty (Ω x))).
+  Proof.
+    iIntros "H".
+    iDestruct (big_sepS_elem_of_acc _ _ x with "H") as "($ & _)";
+      first apply elem_of_fin_to_set.
+  Qed.
+
+  Lemma compat_pair {S1 S2 : Set}
+    `{!EqDecision S1} `{!Finite S1}
+    `{!EqDecision S2} `{!Finite S2}
+    `{!EqDecision (S1 + S2)} `{!Finite (S1 + S2)}
+    (Ω1 : S1 → ty) (Ω2 : S2 → ty) α β τ1 τ2 :
+    ⊢ valid1 Ω1 α τ1 -∗
+      valid1 Ω2 β τ2 -∗
+      valid1 (sum_map' Ω1 Ω2) (interp_pair α β ◎ interp_scope_split) (tPair τ1 τ2).
+  Proof.
+    Opaque pairITV.
+    iIntros "H1 H2".
+    iIntros (αs) "#Hctx Has".
+    cbn-[interp_pair].
+    rewrite ssubst_valid_app.
+    iDestruct "Has" as "[Ha1 Ha2]". cbn-[interp_app].
+    iSpecialize ("H1"  with "Hctx Ha1").
+    iSpecialize ("H2"  with "Hctx Ha2").
+    iApply (expr_pred_bind with "H2").
+    iIntros (βv) "Hb". simpl.
+    rewrite -> get_val_ITV. simpl.
+    iApply (expr_pred_bind with "H1").
+    iIntros (αv) "Ha". simpl.
+    rewrite -> get_val_ITV. simpl.
+    iApply expr_pred_ret.
+    simpl.
+    iExists _,_.
+    by iFrame.
+  Qed.
+
+  Lemma compat_destruct {S1 S2 : Set}
+    `{!EqDecision S1} `{!Finite S1}
+    `{!EqDecision S2} `{!Finite S2}
+    `{!EqDecision (S1 + S2)} `{!Finite (S1 + S2)}
+    (Ω1 : S1 → ty) (Ω2 : S2 → ty)
+    α β τ1 τ2 τ :
+    ⊢ valid1 Ω1 α (tPair τ1 τ2)
+      -∗ valid1 (Ω2 ▹ τ2 ▹ τ1) β τ
+      -∗ valid1 (sum_map' Ω1 Ω2) (interp_destruct α β ◎ interp_scope_split) τ.
+  Proof.
+    Opaque pairITV thunked thunkedV projIT1 projIT2.
+    iIntros "H1 H2".
+    iIntros (αs) "#Hctx Has".
+    cbn-[interp_destruct].
+    rewrite ssubst_valid_app.
+    iDestruct "Has" as "[Ha1 Ha2]".
+    iSpecialize ("H1"  with "Hctx Ha1").
+    iApply (expr_pred_bind (LETCTX _) with "H1").
+    iIntros (αv) "Ha". unfold LETCTX. simpl.
+    rewrite LET_Val/=.
+    iDestruct "Ha" as (β1 β2) "[#Ha [Hb1 Hb2]]".
+    iIntros (x) "Hx".
+    iApply wp_let.
+    iApply (wp_Thunk with "Hctx").
+    {
+      repeat intro; simpl.
+      repeat f_equiv.
+      intro; simpl.
+      f_equiv.
+      intro B; simpl.
+      destruct B as [| [|]]; [by f_equiv | reflexivity | reflexivity].
+    }
+    iNext. iIntros (l1) "Hl1". simpl.
+    iApply wp_let.
+    { solve_proper. }
+    iApply (wp_Thunk with "Hctx").
+    {
+      repeat intro; simpl.
+      repeat f_equiv.
+      intro B; simpl.
+      destruct B as [| [|]]; [reflexivity | by f_equiv | reflexivity].
+    }
+    iNext. iIntros (l2) "Hl2". simpl.
+    pose (ss' := (extend_scope
+                    (extend_scope
+                       (interp_scope_split αs).2
+                       (IT_of_V (thunkedV (projIT2 (IT_of_V αv)) l2)))
+                    (IT_of_V (thunkedV (projIT1 (IT_of_V αv)) l1)))).
+    iSpecialize ("H2" $! ss'
+                  with "Hctx [-Hx] Hx").
+    {
+      iApply ssubst_valid_cons.
+      iSplitR "Hl1 Hb1".
+      - iApply ssubst_valid_cons.
+        iSplitL "Ha2"; first done.
+        Transparent thunkedV thunked.
+        simpl.
+        iIntros (z) "Hz".
+        simpl.
+        iApply wp_val.
+        iModIntro.
+        iExists z; iFrame.
+        iApply wp_lam.
+        iNext.
+        simpl.
+        iApply (wp_bind _ (IFSCtx _ _)).
+        iApply (wp_read with "Hctx Hl2").
+        iNext. iNext. iIntros "Hl2".
+        iApply wp_val. iModIntro.
+        unfold IFSCtx. simpl.
+        rewrite IF_False; last lia.
+        iApply wp_seq.
+        { solve_proper. }
+        iApply (wp_write with "Hctx Hl2").
+        iNext. iNext. iIntros "Hl2".
+        iRewrite "Ha".
+        simpl.
+        rewrite projIT2_pairV.
+        do 3 (iApply wp_tick; iNext).
+        iApply wp_val. iModIntro.
+        iApply "Hb2".
+      - Transparent thunkedV thunked.
+        simpl.
+        iIntros (z) "Hz".
+        simpl.
+        iApply wp_val.
+        iModIntro.
+        iExists z; iFrame.
+        iApply wp_lam.
+        iNext.
+        simpl.
+        iApply (wp_bind _ (IFSCtx _ _)).
+        iApply (wp_read with "Hctx Hl1").
+        iNext. iNext. iIntros "Hl1".
+        iApply wp_val. iModIntro.
+        unfold IFSCtx. simpl.
+        rewrite IF_False; last lia.
+        iApply wp_seq.
+        { solve_proper. }
+        iApply (wp_write with "Hctx Hl1").
+        iNext. iNext. iIntros "Hl1".
+        iRewrite "Ha".
+        simpl.
+        rewrite projIT1_pairV.
+        do 3 (iApply wp_tick; iNext).
+        iApply wp_val. iModIntro.
+        iApply "Hb1".
+    }
+    iApply "H2".
+  Qed.
+
+  Lemma compat_alloc {S : Set}
+    `{!EqDecision S} `{!Finite S}
+    (Ω : S → ty) α τ:
+    ⊢ valid1 Ω α τ -∗
+      valid1 Ω (interp_alloc α) (tRef τ).
+  Proof.
+    iIntros "H".
+    iIntros (αs) "#Hctx Has".
+    iSpecialize ("H" with "Hctx Has").
+    simpl. iApply (expr_pred_bind (LETCTX _) with "H").
+    iIntros (αv) "Hav". unfold LETCTX. simpl.
+    rewrite LET_Val/=.
+    iApply expr_pred_frame.
+    iApply (wp_alloc with "Hctx").
+    iNext. iNext. iIntros (l) "Hl".
+    iApply wp_val. iModIntro. simpl.
+    iExists l.
+    iSplit; first done.
+    iExists αv.
+    iFrame "Hl".
+    iFrame.
+  Qed.
+
+  Lemma compat_replace {S1 S2 : Set}
+    `{!EqDecision S1} `{!Finite S1}
+    `{!EqDecision S2} `{!Finite S2}
+    `{!EqDecision (S1 + S2)} `{!Finite (S1 + S2)}
+    (Ω1 : S1 → ty) (Ω2 : S2 → ty) α β τ τ' :
+    ⊢ valid1 Ω1 α (tRef τ) -∗
+      valid1 Ω2 β τ' -∗
+      valid1 (sum_map' Ω1 Ω2) (interp_replace α β ◎ interp_scope_split) (tPair τ (tRef τ')).
+  Proof.
+    Opaque pairITV.
+    iIntros "H1 H2".
+    iIntros (αs) "#Hctx Has".
+    cbn-[interp_replace].
+    rewrite ssubst_valid_app.
+    iDestruct "Has" as "[Ha1 Ha2]". cbn-[interp_app].
+    iSpecialize ("H1"  with "Hctx Ha1").
+    iSpecialize ("H2"  with "Hctx Ha2").
+    iApply (expr_pred_bind (LETCTX _) with "H2").
+    iIntros (βv) "Hb". unfold LETCTX. simpl.
+    rewrite LET_Val/=.
+    iApply (expr_pred_bind with "H1").
+    iIntros (αv) "Ha". simpl.
+    iDestruct "Ha" as (l) "[Ha Ha']".
+    iDestruct "Ha'" as (γ) "[Hl Hg]".
+    iApply expr_pred_frame.
+    iRewrite "Ha". simpl.
+    rewrite IT_of_V_Ret.
+    rewrite -> get_ret_ret; simpl.
+    iApply wp_let.
+    { solve_proper. }
+    iApply (wp_read with "Hctx Hl").
+    iNext. iNext. iIntros "Hl".
+    iApply wp_val. iModIntro.
+    simpl. iApply wp_seq.
+    { solve_proper. }
+    iApply (wp_write with "Hctx Hl").
+    iNext. iNext. iIntros "Hl".
+    rewrite get_val_ITV. simpl.
+    rewrite get_val_ITV. simpl.
+    iApply wp_val. iModIntro.
+    iExists γ, (RetV l).
+    iSplit; first done.
+    iFrame. eauto with iFrame.
+  Qed.
+
+  Lemma compat_dealloc {S : Set}
+    `{!EqDecision S} `{!Finite S}
+    (Ω : S → ty) α τ:
+    ⊢ valid1 Ω α (tRef τ) -∗
+      valid1 Ω (interp_dealloc α) tUnit.
+  Proof.
+    iIntros "H".
+    iIntros (αs) "#Hctx Has".
+    iSpecialize ("H" with "Hctx Has").
+    iApply (expr_pred_bind with "H").
+    iIntros (αv) "Ha /=".
+    iDestruct "Ha" as (l) "[Ha Ha']".
+    iDestruct "Ha'" as (βv) "[Hl Hb]".
+    iRewrite "Ha". iApply expr_pred_frame. simpl.
+    rewrite IT_of_V_Ret. rewrite -> get_ret_ret. simpl.
+    iApply (wp_dealloc with "Hctx Hl").
+    iNext. iNext. eauto with iFrame.
+  Qed.
+
+  Lemma compat_bool {S : Set}
+    `{!EqDecision S} `{!Finite S}
+    b (Ω : S → ty) :
+    ⊢ valid1 Ω (interp_litbool b) tBool.
+  Proof.
+    iIntros (αs) "#Hctx Has".
+    iApply expr_pred_ret.
+    destruct b; simpl; eauto.
+  Qed.
+
+  Lemma compat_nat {S : Set}
+    `{!EqDecision S} `{!Finite S}
+    n (Ω : S → ty) :
+    ⊢ valid1 Ω (interp_litnat n) tInt.
+  Proof.
+    iIntros (αs) "#Hctx Has".
+    iApply expr_pred_ret. eauto with iFrame.
+  Qed.
+
+  Lemma compat_unit {S : Set}
+    `{!EqDecision S} `{!Finite S}
+    (Ω : S → ty) :
+    ⊢ valid1 Ω interp_litunit tUnit.
+  Proof.
+    iIntros (αs) "#Hctx Has".
+    iApply expr_pred_ret. eauto with iFrame.
+  Qed.
+
+  Lemma compat_var {S : Set}
+    `{!EqDecision S} `{!Finite S}
+    Ω (v : S) :
+    ⊢ valid1 Ω (Force ◎ interp_var v) (Ω v).
+  Proof.
+    iIntros (ss) "#Hctx Has".
+    iIntros (x) "Hx".
+    unfold Force.
+    simpl.
+    iApply (wp_bind rs (AppRSCtx (ss v))).
+    { solve_proper. }
+    iApply wp_val.
+    iModIntro.
+    unfold AppRSCtx.
+    iApply (wp_bind rs (AppLSCtx (IT_of_V (RetV 0)))).
+    { solve_proper. }
+    unfold AppLSCtx.
+    simpl.
+    unfold ssubst_valid.
+    iDestruct (ssubst_valid_lookup _ _ v with "Has Hx") as "Has".
+    iApply (wp_wand with "Has").
+    iIntros (w) "(%y & Hw1 & Hw2)"; simpl.
+    iModIntro.
+    rewrite IT_of_V_Ret.
+    iApply (wp_wand with "Hw1 [Hw2]").
+    iIntros (z) "Hz".
+    iModIntro.
+    iExists y.
+    iFrame.
+  Qed.
+
+  Lemma compat_app {S1 S2 : Set}
+    `{!EqDecision S1} `{!Finite S1}
+    `{!EqDecision S2} `{!Finite S2}
+    `{!EqDecision (S1 + S2)} `{!Finite (S1 + S2)}
+    (Ω1 : S1 → ty) (Ω2 : S2 → ty)
+    α β τ1 τ2 :
+    ⊢ valid1 Ω1 α (tArr τ1 τ2) -∗
+      valid1 Ω2 β τ1 -∗
+      valid1 (sum_map' Ω1 Ω2) (interp_app α β ◎ interp_scope_split) τ2.
+  Proof.
+    iIntros "H1 H2".
+    iIntros (αs) "#Hctx Has".
+    iEval(cbn-[interp_app]).
+    rewrite ssubst_valid_app.
+    iDestruct "Has" as "[Ha1 Ha2]". cbn-[interp_app].
+    iSpecialize ("H1"  with "Hctx Ha1").
+    iSpecialize ("H2"  with "Hctx Ha2").
+    Local Opaque Thunk.
+    iSimpl.
+    iApply (expr_pred_bind (LETCTX _) with "H2").
+    iIntros (βv) "H2". unfold LETCTX. iSimpl.
+    rewrite LET_Val/=.
+    iApply (expr_pred_bind (LETCTX _) with "H1").
+    iIntros (αv) "H1". unfold LETCTX. iSimpl.
+    rewrite LET_Val/=.
+    by iApply "H1".
+  Qed.
+
+  Lemma compat_lam {S : Set}
+    `{!EqDecision S} `{!Finite S}
+    (Ω : S → ty) τ1 τ2 α :
+    ⊢ valid1 (Ω ▹ τ1) α τ2 -∗
+      valid1 Ω (interp_lam α) (tArr τ1 τ2).
+  Proof.
+    iIntros "H".
+    iIntros (αs) "#Hctx Has".
+    iIntros (x) "Hx".
+    iApply wp_val.
+    iModIntro. simpl.
+    iExists _; iFrame.
+    iIntros (βv) "Hb". clear x.
+    iIntros (x) "Hx".
+    iApply (wp_bind _ (AppRSCtx _)).
+    Local Transparent Thunk.
+    Local Opaque thunked thunkedV.
+    iSimpl. iApply (wp_alloc with "Hctx").
+    { solve_proper. }
+    iNext. iNext. iIntros (l) "Hl".
+    iApply wp_val. iModIntro.
+    unfold AppRSCtx.
+    iApply wp_lam. iNext.
+    iEval(cbn-[thunked]).
+    pose (ss' := extend_scope αs (IT_of_V (thunkedV (IT_of_V βv) l))).
+    iSpecialize ("H" $! ss'
+             with "Hctx [-Hx] Hx").
+    {
+      iApply ssubst_valid_cons.
+      iFrame "Has".
+      Local Transparent thunked thunkedV.
+      simpl.
+      iIntros (x') "Hx".
+      iApply wp_val.
+      iModIntro.
+      iExists x'.
+      iFrame "Hx".
+      iApply wp_lam.
+      iNext.
+      iApply (wp_bind _ (IFSCtx _ _)).
+      iApply (wp_read with "Hctx Hl").
+      iNext. iNext. iIntros "Hl".
+      iApply wp_val. iModIntro.
+      unfold IFSCtx. simpl.
+      rewrite IF_False; last lia.
+      iApply wp_seq.
+      { solve_proper. }
+      iApply (wp_write with "Hctx Hl").
+      iNext. iNext. iIntros "Hl".
+      iApply wp_val. iModIntro.
+      iApply "Hb".
+    }
+    iApply "H".
+  Qed.
+
+  Lemma fundamental_affine (S : Set)
+    {HE : EqDecision S} {HF : Finite S}
+    (Ω : S → ty)
+    (e : expr S) τ :
+    typed Ω e τ →
+    ⊢ valid1 Ω (interp_expr _ e) τ.
+  Proof.
+    intros H.
+    induction H.
+    - by iApply compat_var.
+    - iApply compat_lam;
+        iApply IHtyped.
+    - iApply (@compat_app S1 S2 EqDecisionLeft FiniteLeft EqDecisionRight FiniteRight).
+      + iApply IHtyped1.
+      + iApply IHtyped2.
+    - iApply (@compat_pair S1 S2 EqDecisionLeft FiniteLeft EqDecisionRight FiniteRight).
+      + iApply IHtyped1.
+      + iApply IHtyped2.
+    - iApply (@compat_destruct S1 S2 EqDecisionLeft FiniteLeft EqDecisionRight FiniteRight).
+      + iApply IHtyped1.
+      + iApply IHtyped2.
+    - iApply compat_alloc;
+        iApply IHtyped.
+    - iApply (@compat_replace S1 S2 EqDecisionLeft FiniteLeft EqDecisionRight FiniteRight).
+      + iApply IHtyped1.
+      + iApply IHtyped2.
+    - iApply compat_dealloc;
+        iApply IHtyped.
+    - by iApply compat_nat.
+    - by iApply compat_bool.
+    - by iApply compat_unit.
+  Qed.
+
+End logrel.
+
+Arguments interp_tarr {_ _ _ _ _ _ _ _ _ _ _ _ _} Φ1 Φ2.
+Arguments interp_tbool {_ _ _ _ _ _}.
+Arguments interp_tnat {_ _ _ _ _ _}.
+Arguments interp_tunit {_ _ _ _ _ _}.
+Arguments interp_ty {_ _ _ _ _ _ _ _ _ _ _ _ _ _ _} τ.
+
+Local Definition rs : gReifiers NotCtxDep 2 :=
+  gReifiers_cons NotCtxDep reify_store (gReifiers_cons NotCtxDep input_lang.interp.reify_io (gReifiers_nil NotCtxDep)).
+
+Variable Hdisj : ∀ (Σ : gFunctors) (P Q : iProp Σ), disjunction_property P Q.
+
+Require Import gitrees.gitree.greifiers.
+
+Program Definition ı_scope R `{!Cofe R} : @interp_scope (gReifiers_ops NotCtxDep rs) R _ Empty_set := λne (x : ∅), match x with end.
+
+Lemma logrel1_adequacy cr Σ R `{!Cofe R, !SubOfe natO R, !SubOfe unitO R, !SubOfe locO R} `{!invGpreS Σ}
+  `{!statePreG rs R Σ} `{!heapPreG rs R Σ} τ
+  (α : interp_scope ∅ -n>  IT (gReifiers_ops NotCtxDep rs) R) (β : IT (gReifiers_ops NotCtxDep rs) R) st st' k :
+  (∀ `{H1 : !invGS Σ} `{H2: !stateG rs R Σ} `{H3: !heapG rs R Σ},
+      (£ cr ⊢ valid1 rs notStuck (λne _: unitO, True)%I □ α τ)%I) →
+  ssteps (gReifiers_sReifier NotCtxDep rs) (α (ı_scope _)) st β st' k →
+  (∃ β1 st1, sstep (gReifiers_sReifier NotCtxDep rs) β st' β1 st1)
+   ∨ (∃ βv, IT_of_V βv ≡ β).
+Proof.
+  intros Hlog Hst.
+  destruct (IT_to_V β) as [βv|] eqn:Hb.
+  { right. exists βv. apply IT_of_to_V'. rewrite Hb; eauto. }
+  left.
+  cut ((∃ β1 st1, sstep (gReifiers_sReifier NotCtxDep rs) β st' β1 st1)
+      ∨ (∃ e, β ≡ Err e ∧ notStuck e)).
+  { intros [?|He]; first done.
+    destruct He as [? [? []]]. }
+  eapply (wp_safety (S cr)); eauto.
+  { apply Hdisj. }
+  { by rewrite Hb. }
+  intros H1 H2.
+  exists (λ _, True)%I. split.
+  { apply _. }
+  iIntros "[[Hone Hcr] Hst]".
+  pose (σ := st.1).
+  pose (ios := st.2.1).
+  iMod (new_heapG rs σ) as (H3) "H".
+  iAssert (has_substate σ ∗ has_substate ios)%I with "[Hst]" as "[Hs Hio]".
+  { unfold has_substate, has_full_state.
+    assert (of_state NotCtxDep rs (IT (gReifiers_ops NotCtxDep rs) _) st ≡
+            of_idx NotCtxDep rs (IT (gReifiers_ops NotCtxDep rs) _) sR_idx (sR_state σ)
+            ⋅ of_idx NotCtxDep rs (IT (gReifiers_ops NotCtxDep rs) _) sR_idx (sR_state ios)) as ->; last first.
+    { rewrite -own_op. done. }
+    unfold sR_idx. simpl.
+    intro j.
+    rewrite discrete_fun_lookup_op.
+    inv_fin j.
+    { unfold of_state, of_idx. simpl.
+      erewrite (eq_pi _ _ _ (@eq_refl _ 0%fin)). done. }
+    intros j. inv_fin j.
+    { unfold of_state, of_idx. simpl.
+      erewrite (eq_pi _ _ _ (@eq_refl _ 1%fin)). done. }
+    intros i. inversion i. }
+  iApply fupd_wp.
+  iMod (inv_alloc (nroot.@"storeE") _ (∃ σ, £ 1 ∗ has_substate σ ∗ own (heapG_name rs) (●V σ))%I with "[-Hcr]") as "#Hinv".
+  { iNext. iExists _. iFrame. }
+  simpl.
+  iPoseProof (@Hlog _ _ _ with "Hcr") as "Hlog".
+  iSpecialize ("Hlog" $! (ı_scope _) with "Hinv []").
+  { iApply ssubst_valid_empty. }
+  iSpecialize ("Hlog" $! tt with "[//]").
+  iModIntro.
+  iApply (wp_wand with "Hlog").
+  eauto with iFrame.
+Qed.
+
+Definition R := sumO locO (sumO unitO natO).
+
+Lemma logrel1_safety e τ (β : IT (gReifiers_ops NotCtxDep rs) R) st st' k :
+  typed □ e τ →
+  ssteps (gReifiers_sReifier NotCtxDep rs) (interp_expr rs e (ı_scope _)) st β st' k →
+  (∃ β1 st1, sstep (gReifiers_sReifier NotCtxDep rs) β st' β1 st1)
+   ∨ (∃ βv, IT_of_V βv ≡ β).
+Proof.
+  intros Hty Hst.
+  pose (Σ:=#[invΣ;stateΣ rs R;heapΣ rs R]).
+  eapply (logrel1_adequacy 0 Σ); eauto; try apply _.
+  iIntros (? ? ?) "_".
+  iApply (fundamental_affine rs notStuck (λne _ : unitO, True)%I).
+  apply Hty.
+Qed.
