theories/examples/input_lang_callcc/logrel.v
@@ -1,6 +1,6 @@
 (** Logical relation for adequacy for the IO lang *)
 From gitrees Require Import gitree.
-From gitrees.input_lang_callcc Require Import lang interp hom.
+From gitrees.examples.input_lang_callcc Require Import lang interp hom.
 Require Import gitrees.lang_generic.
 Require Import Binding.Lib Binding.Set Binding.Env.
 
